theories/VLSM/Core/VLSMProjections.v
@@ -2671,12 +2671,37 @@ Context
   (X : VLSM message)
   .
 
+Lemma pre_loaded_vlsm_incl_relaxed
+  (P Q : message -> Prop)
+  (PimpliesQorValid : forall m : message, P m -> Q m \/ valid_message_prop (pre_loaded_vlsm X Q) m)
+  : VLSM_incl (pre_loaded_vlsm X P) (pre_loaded_vlsm X Q).
+Proof.
+  apply basic_VLSM_incl.
+  - cbv; intuition.
+  - intros _ _ m _ _ [Him | Hp].
+    + apply initial_message_is_valid. left. assumption.
+    + apply PimpliesQorValid in Hp as [Hq | Hvalid]; [|assumption].
+      apply initial_message_is_valid. right. assumption.
+  - cbv; intuition.
+  - cbv; intuition.
+Qed.
+
 Lemma pre_loaded_vlsm_incl
   (P Q : message -> Prop)
   (PimpliesQ : forall m : message, P m -> Q m)
   : VLSM_incl (pre_loaded_vlsm X P) (pre_loaded_vlsm X Q).
 Proof.
-  apply basic_VLSM_incl_preloaded_with; cbv; intuition.
+  apply pre_loaded_vlsm_incl_relaxed. intuition.
+Qed.
+
+Lemma pre_loaded_vlsm_with_valid_eq
+  (P Q : message -> Prop)
+  (QimpliesValid : forall m, Q m -> valid_message_prop (pre_loaded_vlsm X P) m)
+  : VLSM_eq (pre_loaded_vlsm X (fun m => P m \/ Q m)) (pre_loaded_vlsm X P).
+Proof.
+  apply VLSM_eq_incl_iff; split.
+  - apply pre_loaded_vlsm_incl_relaxed. intuition.
+  - cbv; apply pre_loaded_vlsm_incl. intuition.
 Qed.
 
 Lemma pre_loaded_vlsm_idem_l
